thy/Bool_Func.thy
@@ -37,7 +37,8 @@ text\<open>All of these are implemented and had their implementation verified.\<
 definition "bf_imp a b = bf_ite a b bf_True"
 lemma bf_imp_alt: "bf_imp a b = bf_or (bf_not a) b" unfolding bf_or_def bf_not_def bf_imp_def unfolding bf_ite_def bf_True_def bf_False_def unfolding fun_eq_iff by simp
 
-lemma [dest!]: "bf_False = bf_True \<Longrightarrow> False" unfolding bf_True_def bf_False_def fun_eq_iff by simp (* Occurs here and there as goal for sep_auto *)
+lemma [dest!,elim!]: "bf_False = bf_True \<Longrightarrow> False" "bf_True = bf_False \<Longrightarrow> False" unfolding bf_True_def bf_False_def fun_eq_iff by simp_all (* Occurs here and there as goal for sep_auto *)
+lemma [dest!,elim!]: "(\<lambda>_. False) = (\<lambda>_. True) \<Longrightarrow> False" "(\<lambda>_. True) = (\<lambda>_. False) \<Longrightarrow> False" unfolding bf_True_def bf_False_def fun_eq_iff by simp_all
 
 lemmas [simp] = bf_and_def bf_or_def bf_nand_def bf_biimp_def bf_xor_alt bf_nor_def bf_not_def 
 
